

$$1.1) \quad \mathcal{V} = \{v \in H^1(\Omega) : v|_{\Gamma_0} = 0\}$$

$$u = u_0 + R_g, \quad R_g: \Omega \rightarrow \mathbb{R} \text{ s.t. } R_g = g \text{ on } \Gamma_D$$

$$(PW) \text{ Find } u_0 \in \mathcal{V} \text{ s.t.}$$

$$\Rightarrow \int_{\Omega} -\mu \Delta u \cdot v \, dx + \int_{\Omega} \bar{b} \cdot \nabla u \cdot \nabla v \, dx + \int_{\Omega} \sigma u v \, dx = \int_{\Omega} f v \, dx$$

$$\Rightarrow \int_{\Omega} \mu \nabla u \cdot \nabla v \, dx - \int_{\Gamma_N} \mu \nabla u \bar{n} \cdot v \, dx - \int_{\Omega} \bar{b} u \cdot \nabla v \, dx + \int_{\Gamma_N} b u \bar{n} v \, dx + \int_{\Omega} \sigma u v \, dx = \int_{\Omega} f v \, dx$$

$$\Rightarrow \int_{\Omega} \mu \nabla u \nabla v \, dx - \int_{\Gamma_N} (\underbrace{\mu \nabla u \bar{n} - \bar{b} u}_{\phi}) v \, dx - \int_{\Omega} \bar{b} u \cdot \nabla v \, dx + \int_{\Omega} \sigma u v \, dx = \int_{\Omega} f v \, dx$$

$$\Rightarrow \underbrace{\int_{\Omega} \mu \nabla u \nabla v - \int_{\Omega} \bar{b} u \cdot \nabla v \, dx + \int_{\Omega} \sigma u v \, dx}_{a(u, v)} = \underbrace{\int_{\Omega} f v \, dx + \int_{\Gamma_N} \phi v \, dx}_{F(v)}$$

$$\Rightarrow a(u, v) = F(v) \xrightarrow[u = u_0 + R_g]{} a(u_0, v) = F(v) - a(R_g, v) = \tilde{F}(v)$$

$$1.6) \quad \phi_1 = \phi|_{\Gamma_1}, \quad n = \vec{x}$$

$$\mu \frac{\partial u}{\partial x} - b \cdot \begin{pmatrix} 1 \\ 0 \end{pmatrix} u = \phi_1 \quad \text{on } \Gamma_1$$

$$\mu - b_1(x+y) = \phi_1$$

$$\phi_1 = \mu - b_1(1+y)$$

$$\phi_3 = \phi|_{\Gamma_3}$$

$$\mu \frac{\partial u}{\partial y} - b \cdot \begin{pmatrix} 0 \\ 1 \end{pmatrix} u = \phi_3$$

$$\mu - b_2(x+y) = \phi_3$$

$$\phi_3 = \mu - b_2(x+1)$$

$$F = b_1 + b_2 + \sigma(x+y)$$

$$\operatorname{div}(\nabla u) = \frac{\partial^2 u}{\partial x^2} + \frac{\partial^2 u}{\partial y^2} = 0; \quad -\operatorname{div}(\mu \nabla u) = 0$$

$$\nabla u = \begin{pmatrix} 1 \\ 1 \end{pmatrix}; \quad \operatorname{div}(b u) = \bar{b} \cdot \nabla u = b_1 + b_2$$

$$u = x+y; \quad \sigma u = \sigma(x+y)$$

$$g(x, y) = u_{ex}(x, y) \text{ on } \Gamma_D$$

$$= x+y$$